theories/memmove.v
@@ -129,11 +129,9 @@ Definition locle_itree : itree (moduleE imp_event unit) unit :=
       TAssume (f = "locle");;;;
       l1 ← TAll loc;;; l2 ← TAll loc;;;
       TAssume (vs = [ValLoc l1; ValLoc l2]);;;;
-      if bool_decide (l1.1 = l2.1) then
-        TVis (Outgoing, EIReturn (ValBool (bool_decide (l1.2 ≤ l2.2))) h)
-      else
-        b ← TExist _;;;
-        TVis (Outgoing, EIReturn (ValBool b) h)).
+      b ← TExist _;;;
+      TAssert (l1.1 = l2.1 → b = bool_decide (l1.2 ≤ l2.2));;;;
+      TVis (Outgoing, EIReturn (ValBool b) h)).
 
 Lemma locle_itree_strong_refines_itree :
   trefines (MS (mod_itree imp_event (gmap prov Z)) (locle_itree_strong, ∅))
@@ -167,10 +165,12 @@ Proof.
   go_i => Hz2. go.
   go_i.
   go_i.
-  case_bool_decide (_ = _) as Heq.
-  - rewrite Heq in Hz2. simplify_map_eq. go_s. split; [| go; by apply: Hloop].
-    repeat case_bool_decide => //; lia.
-  - go_s. eexists _. go. go_s. split!. go. by apply: Hloop.
+  go_s. eexists _. go.
+  go_s. split; [shelve|]. go.
+  go_s. split!. go.
+  by apply: Hloop.
+  Unshelve.
+  - move => Heq. rewrite Heq in Hz2. simplify_map_eq. repeat case_bool_decide; lia.
 Qed.
 
 Lemma locle_asm_refines_itree :
@@ -258,20 +258,29 @@ Definition memmove_imp : fndef := {|
   fd_vars := [];
   fd_body := If (imp.Call "locle" [Var "d"; Var "s"])
                 (imp.Call "memcpy" [Var "d"; Var "s"; Var "n"; Val $ ValNum 1])
-                (imp.Call "memcpy" [BinOp (Var "d") AddOp (BinOp (Var "n") AddOp (Val $ ValNum (-1)));
-                                    BinOp (Var "s") AddOp (BinOp (Var "n") AddOp (Val $ ValNum (-1)));
-                                    Var "n"; Val $ ValNum (-1)]);
+                (LetE "d'" (BinOp (Var "d") ShiftOp (BinOp (Var "n") AddOp (Val $ ValNum (-1)))) $
+                 LetE "s'" (BinOp (Var "s") ShiftOp (BinOp (Var "n") AddOp (Val $ ValNum (-1)))) $
+                 imp.Call "memcpy" [Var "d'"; Var "s'"; Var "n"; Val $ ValNum (-1)]);
   fd_static := I
 |}.
+Definition memmove_prog : gmap string fndef :=
+  <["memmove" := memmove_imp]> $ ∅.
+
 
 Definition memcpy_imp : fndef := {|
-  fd_args := ["d"; "s"; "n"];
+  fd_args := ["d"; "s"; "n"; "o"];
   fd_vars := [];
-  fd_body := If (imp.Call "locle" [Var "d"; Var "s"])
-                (imp.Call "memcpy" [Var "d"; Var "s"; Var "n"; Val $ ValNum 1])
-                (imp.Call "memcpy" [Var "d"; Var "s"; Var "n"; Val $ ValNum (-1)]);
+  fd_body := If (BinOp (Val $ ValNum 0) LtOp (Var "n"))
+               (LetE "_" (Store (Var "d") (Load (Var "s"))) $
+                LetE "d'" (BinOp (Var "d") ShiftOp (Var "o")) $
+                LetE "s'" (BinOp (Var "s") ShiftOp (Var "o")) $
+                LetE "n'" (BinOp (Var "n") AddOp (Val $ ValNum (-1))) $
+                imp.Call "memcpy" [Var "d'"; Var "s'"; Var "n'"; Var "o"])
+               (Val 0);
   fd_static := I
 |}.
+Definition memcpy_prog : gmap string fndef :=
+  <["memcpy" := memcpy_imp]> $ ∅.
 
 Definition main_imp : fndef := {|
   fd_args := [];
@@ -286,6 +295,8 @@ Definition main_imp : fndef := {|
              (Val $ ValNum 0);
   fd_static := I
 |}.
+Definition main_prog : gmap string fndef :=
+  <["main" := main_imp]> $ ∅.
 
 Definition main_f2i : gmap string Z :=
   <["main" := 50]> $
@@ -309,7 +320,7 @@ Definition memcpy_asm : gmap Z asm_instr :=
 Lemma main_asm_refines_imp :
   trefines (MS asm_module (initial_asm_state main_asm))
            (MS (imp_to_asm (dom _ main_asm) {["main"]} main_f2i imp_module)
-               (initial_imp_to_asm_state ∅ imp_module (initial_imp_state (<["main" := main_imp]> ∅)))).
+               (initial_imp_to_asm_state ∅ imp_module (initial_imp_state main_prog))).
 Proof.
   apply: compile_correct; [|done|..].
   - by vm_compute.
@@ -321,7 +332,7 @@ Qed.
 Lemma memmove_asm_refines_imp :
   trefines (MS asm_module (initial_asm_state memmove_asm))
            (MS (imp_to_asm (dom _ memmove_asm) {["memmove"]} main_f2i imp_module)
-               (initial_imp_to_asm_state ∅ imp_module (initial_imp_state (<["memmove" := memmove_imp]> ∅)))).
+               (initial_imp_to_asm_state ∅ imp_module (initial_imp_state memmove_prog))).
 Proof.
   apply: compile_correct; [|done|..].
   - by vm_compute.
@@ -333,11 +344,196 @@ Qed.
 Lemma memcpy_asm_refines_imp :
   trefines (MS asm_module (initial_asm_state memcpy_asm))
            (MS (imp_to_asm (dom _ memcpy_asm) {["memcpy"]} main_f2i imp_module)
-               (initial_imp_to_asm_state ∅ imp_module (initial_imp_state (<["memcpy" := memcpy_imp]> ∅)))).
+               (initial_imp_to_asm_state ∅ imp_module (initial_imp_state memcpy_prog))).
 Proof.
   apply: compile_correct; [|done|..].
   - by vm_compute.
   - by vm_compute.
   - move => ??. rewrite /main_f2i/locle_f2i !lookup_insert_Some !lookup_empty.
     move => ?. destruct_all?; simplify_eq; compute_done.
+Qed.
+
+Lemma memcpy_spec n0 d s d' s' n o K e h m σ1 σ2 b cs hvs `{!ImpExprFill e K
+      (imp.Call "memcpy" [Val (ValLoc d); Val (ValLoc s); Val (ValNum n); Val o])}:
+  n = Z.of_nat (length hvs) →
+  o = 1 ∨ o = -1 →
+  d' = (if bool_decide (o = 1) then d else d +ₗ (- n + 1)) →
+  s' = (if bool_decide (o = 1) then s else s +ₗ (- n + 1)) →
+  (if bool_decide (o = 1) then d.1 = s.1 → d.2 ≤ s.2 else d.1 = s.1 → s.2 ≤ d.2) →
+  (∀ i v, hvs !! i = Some v → h_heap h !! (s' +ₗ Z.of_nat i) = Some v) →
+  (∀ i v, hvs !! i = Some v → heap_alive h (d' +ₗ Z.of_nat i)) →
+  ((MLFLeft, cs, Imp (expr_fill K (Val (ValNum 0)))
+                   (heap_update_big h (kmap (λ i, d' +ₗ i) (map_seqZ 0 hvs)))
+                   (memmove_prog ∪ memcpy_prog), σ1)
+    ⪯{imp_prod {["memmove"; "memcpy"]} {["locle"]} imp_module (mod_itree imp_event ()), m, n0, true}
+  σ2) →
+  (MLFLeft, cs, Imp e h (memmove_prog ∪ memcpy_prog), σ1)
+    ⪯{imp_prod {["memmove"; "memcpy"]} {["locle"]} imp_module (mod_itree imp_event ()), m, n0, b}
+  σ2.
+Proof.
+  elim/ti_lt_ind: n0 b d d' s s' n h hvs e K ImpExprFill0 => n1 IH b d d' s s' n h hvs e K [->] ? Ho ?? Hle Hhvs Halive Hcont. subst.
+  tstep_i. split! => *. simplify_map_eq. split!. rewrite orb_true_r.
+  tstep_i. move => ?? [??]. simplify_eq. split!.
+  tstep_i. split!.
+  tstep_i. case_bool_decide (_ < _). 2: {
+    tstep_i. split!. destruct hvs; [|done]. simplify_eq/=.
+    move: Hcont. rewrite kmap_empty heap_update_big_empty. done.
+  }
+  destruct Ho; simplify_eq/=; repeat case_bool_decide => //.
+  - destruct hvs; [done|].
+    have := Hhvs 0%nat _ ltac:(done). rewrite shift_loc_0 => ?.
+    have := Halive 0%nat _ ltac:(done). rewrite shift_loc_0 => ?.
+    tstep_i. split!.
+    tstep_i. split!.
+    tstep_i.
+    tstep_i.
+    tstep_i.
+    tstep_i.
+    tstep_i.
+    tstep_i.
+    tstep_i.
+    have ->: (S (length hvs) + -1) = (length hvs) by lia.
+    apply: tsim_mono_to_tiS => ??. apply: IH; [done|eauto_tstep|done|by left|done|done|..].
+    { move => /=. lia. }
+    { move => i v' ? /=. rewrite -shift_loc_S.
+      rewrite lookup_alter_ne; [by apply: Hhvs|].
+      destruct (decide (d.1 = s.1)); [|naive_solver].
+      destruct d, s; rewrite /shift_loc => ?; simplify_eq/=. lia.
+    } { move => ???. apply heap_alive_update. rewrite -shift_loc_S. by apply: Halive. }
+    simpl. tstep_i. split!.
+    move: Hcont.
+    rewrite /= kmap_insert shift_loc_0 heap_update_big_update.
+    rewrite -insert_union_r. 2: {
+      eapply lookup_kmap_None; [by apply _|].
+      rewrite /shift_loc. move => ? /=?. destruct d; simplify_eq/=. apply lookup_map_seqZ_None. lia.
+    }
+    rewrite right_id_L.
+    enough (kmap (λ i : Z, d +ₗ i) (map_seqZ (Z.succ 0) hvs) =@{gmap _ _}
+            kmap (λ i : Z, d +ₗ 1 +ₗ i) (map_seqZ 0 hvs)) as ->. {
+      move => ?. apply: tsim_mono; [done|]. etrans; [|done]. apply ti_le_S.
+    }
+    apply map_eq => i. apply option_eq => v'. rewrite !lookup_kmap_Some.
+    setoid_rewrite lookup_map_seqZ_Some. split; move => [j ?]; destruct_all?; simplify_eq.
+    + eexists (Z.pred j).
+      rewrite Z.sub_pred_l -Z.sub_succ_r. split!; [|lia].
+      rewrite /shift_loc/=. f_equal. lia.
+    + eexists (Z.succ j).
+      rewrite Z.sub_succ_r Z.sub_succ_l Z.pred_succ. split!; [|lia].
+      rewrite /shift_loc/=. f_equal. lia.
+  - destruct (snoc_inv hvs) as [|[v[hvs' ?]]]; [naive_solver|]. simplify_eq. tstep_i.
+    move: Hhvs Halive. rewrite app_length /=.
+    have -> : (- (length hvs' + 1)%nat + 1) = - length hvs' by lia.
+    move => Hhvs Halive.
+    have := Hhvs (length hvs') v.
+    have := Halive (length hvs') v.
+    rewrite lookup_app_r // -minus_n_n /= !shift_loc_add_sub; [|lia..]. move => ??.
+    split!; [naive_solver|].
+    tstep_i. split!; [naive_solver|].
+    tstep_i.
+    tstep_i.
+    tstep_i.
+    tstep_i.
+    tstep_i.
+    tstep_i.
+    tstep_i.
+    have ->: ((length hvs' + 1)%nat + -1) = length hvs' by lia.
+    apply: tsim_mono_to_tiS => ??. apply: IH; [done|eauto_tstep|done|by right|..].
+    { have ->: d +ₗ -1 +ₗ (- length hvs' + 1) = d +ₗ (- length hvs'); [|done].
+      rewrite /shift_loc /=. f_equal. lia. }
+    { have ->: s +ₗ -1 +ₗ (- length hvs' + 1) = s +ₗ (- length hvs'); [|done].
+      rewrite /shift_loc /=. f_equal. lia. }
+    { move => /=. lia. }
+    { move => i v' Hv' /=.  move: (Hv') => /(lookup_lt_Some _ _ _)?.
+      rewrite lookup_alter_ne; [apply: Hhvs; apply lookup_app_Some; naive_solver|].
+      destruct (decide (d.1 = s.1)); [|naive_solver].
+      destruct d, s; rewrite /shift_loc => ?; simplify_eq/=. lia.
+    } { move => ???. apply heap_alive_update. apply: Halive. apply lookup_app_Some; naive_solver. }
+    simpl. tstep_i. split!.
+    move: Hcont.
+    rewrite /= heap_update_big_update app_length /=.
+    have -> : (- (length hvs' + 1)%nat + 1) = - length hvs' by lia.
+    rewrite map_seqZ_app /= kmap_union kmap_insert kmap_empty shift_loc_add_sub //.
+    move => ?. apply: tsim_mono; [done|]. etrans; [|done]. apply ti_le_S.
+Qed.
+
+Definition memmove_itree : itree (moduleE imp_event unit) unit :=
+  ITree.forever (
+    '(f, vs, h) ← TReceive (λ '(f, vs, h), (Incoming, EICall f vs h));;;
+    TAssume (f = "memmove");;;;
+    '(d, s, n) ← TAll _;;;
+    TAssume (vs = [ValLoc d; ValLoc s; ValNum n]);;;;
+    hvs ← TAll (list val);;;
+    TAssume (n = Z.of_nat (length hvs));;;;
+    TAssume (∀ i v, hvs !! i = Some v → h_heap h !! (s +ₗ Z.of_nat i) = Some v);;;;
+    TAssume (∀ i v, hvs !! i = Some v → heap_alive h (d +ₗ Z.of_nat i));;;;
+    TVis (Outgoing, EIReturn 0 (heap_update_big h (kmap (λ i, d +ₗ i) (map_seqZ 0 hvs))) );;;;
+    Ret ()).
+
+Lemma memmove_refines_itree :
+  trefines (MS (imp_prod {["memmove"; "memcpy"]} {["locle"]} imp_module (mod_itree _ _))
+              initial_imp_prod_state imp_module (mod_itree _ _)
+              (initial_imp_state (memmove_prog ∪ memcpy_prog)) (locle_itree, tt))
+           (MS (mod_itree _ _) (memmove_itree, tt)).
+Proof.
+  apply: tsim_implies_trefines => n0 /=.
+  unshelve eapply tsim_remember. { simpl. exact (λ _ '(σi, cs, Imp e h fns, (ti, _)) '(t, _),
+    eqit eq true false ti locle_itree ∧
+    t ≈ memmove_itree ∧
+    cs = [] ∧
+    σi = MLFNone ∧
+    e = Waiting false ∧
+    fns = (memmove_prog ∪ memcpy_prog)). }
+  { split!. } { done. }
+  move => n ? IH [[[??] [???]] [??]] [??] ?. destruct_all?; simplify_eq.
+  tstep_i => *. case_match; destruct_all?; simplify_eq/=.
+  go_s.
+  go_s. eexists (_, _, _). rewrite -/memmove_itree. go.
+  go_s. split!. go.
+  go_s => ?. go.
+  go_s => -[[??]?]. go.
+  go_s => ?. go.
+  go_s => hvs. go.
+  go_s => ?. go.
+  go_s => Hhvs. go.
+  go_s => ?. go.
+  simplify_map_eq/=. case_bool_decide; [|done].
+  tstep_i. split!. move => *. simplify_map_eq.
+  tstep_i. split!. move => ??. simplify_map_eq. split!.
+  tstep_i => *. destruct_all?. simplify_eq/=. split!.
+  tstep_i. split!. move => *. destruct_all?. simplify_eq. repeat case_bool_decide => //.
+  tstep_i. rewrite -/locle_itree. go.
+  go_i => -[[??]?]. go.
+  go_i => *. simplify_eq. go.
+  go_i. split!. go.
+  go_i. eexists _. go.
+  go_i. eexists _. go.
+  go_i. split!. go.
+  go_i => b. go.
+  go_i => Heq. go.
+  go_i => *. destruct_all?. simplify_eq. go.
+  tstep_i. split!. move => *. simplify_eq.
+  tstep_i.
+  destruct b.
+  - apply: memcpy_spec; [eauto_tstep|done|by left|by rewrite bool_decide_true|by rewrite bool_decide_true| |done|done|..].
+    { rewrite bool_decide_true //. case_bool_decide; lia. }
+    simpl. tstep_i. split!.
+    tstep_i. move => *. destruct_all?; simplify_eq/=.
+    go_s. split!. rewrite bind_ret_l. go.
+    eapply IH; [done|]. split!.
+  - tstep_i.
+    tstep_i.
+    tstep_i.
+    tstep_i.
+    tstep_i.
+    tstep_i.
+    apply: memcpy_spec; [eauto_tstep|done|by right|..].
+    { rewrite bool_decide_false; [|done]. rewrite shift_loc_add_sub; [done|lia]. }
+    { rewrite bool_decide_false; [|done]. rewrite shift_loc_add_sub; [done|lia]. }
+    { rewrite bool_decide_false //=. case_bool_decide; lia. }
+    { done. }
+    { done. }
+    simpl. tstep_i. split!.
+    tstep_i. move => *. destruct_all?; simplify_eq/=.
+    go_s. split!. rewrite bind_ret_l. go.
+    eapply IH; [done|]. split!.
 Qed.
